

①

$$L \frac{di}{dt} + Ri_a = e_m(t) - K_b \frac{d\theta_m}{dt}$$

$$L \frac{di}{dt} + Ri_a = e_m(t) - \frac{K_b}{K_R} \frac{d\cancel{\theta}_m}{dt}$$

$$L \frac{di}{dt} + Ri_a = e_m(t) - \frac{K_b}{K_R} \left(\frac{N_2}{N_1} \right) \dot{x}_L$$

$$(Ls + R) I_a(s) = E_m(s) - \frac{K_b}{K_R} \frac{N_2}{N_1} s X_L(s)$$

Eq — ①

$$J_m + J_p = J$$

$$J \frac{d\theta_m^2}{dt^2} + D_1 \frac{d\theta_m}{dt} = T_m$$

$$\frac{J}{K_R} \ddot{x}_m + \frac{D_1}{K_R} \dot{x}_m = K_m I_a$$

$$\frac{J}{K_R} \frac{N_2}{N_1} \ddot{x}_L + \frac{D_1}{K_R} \frac{N_2}{N_1} \dot{x}_L = K_m I_a$$

$$\left(\frac{J}{K_R} \frac{N_2}{N_1} s^2 + \frac{D_1}{K_R} \frac{N_2}{N_1} s \right) X_L(s) = K_m I_a(s)$$

Eq — ②

$$J_2 \ddot{\theta}_L + D_2 \dot{\theta}_L = \tau_L$$

$$J_2 = J_g + J_s$$

(2)

Where,

$$\tau_L = K_s f_L(t)$$

$$\tau_L = K_s [m_L \ddot{x}_L + b \dot{x}_L + d(t)]$$

So,

$$J_2 \ddot{\theta}_L + D_2 \dot{\theta}_L = K_s [m_L \ddot{x}_L + b \dot{x}_L + d(t)]$$

$$\frac{J_2}{K_R} \ddot{x}_L + \frac{D_2}{K_R} \dot{x}_L - K_s m_L \ddot{x}_L - K_s b \dot{x}_L - K_s d(t) = 0$$

$$\left(\frac{J_2}{K_R} - K_s m_L \right) \ddot{x}_L + \left(\frac{D_2}{K_R} - K_s b \right) \dot{x}_L - K_s d(t) = 0$$

$$\left[\left(\frac{J_2}{K_R} - K_s m_L \right) s^2 + \left(\frac{D_2}{K_R} - K_s b \right) s \right] X_L(s) = K_s D(s)$$

eq (3)

eq (2) - eq (3)

$$\underbrace{\left[\left(\frac{J}{K_R} \frac{N_2}{N_1} - \frac{J_2}{K_R} + K_s m_L \right) s^2 + \left(\frac{D_1}{K_R} \frac{N_2}{N_1} - \frac{D_2}{K_R} + K_s b \right) s \right]}_{C_1} X_L(s) = \underbrace{K_m I_a(s) - K_s D(s)}_{C_2}$$

For $\frac{X_L(s)}{E_m(s)} \rightarrow D(s) = 0$

$$I_a(s) = \frac{1}{K_m} [C_1 s^2 + C_2 s] X_L(s) \quad (4)$$

(3)

Put eq. (4) in (1)

$$(Ls + R) \frac{1}{K_m} (C_1 s^2 + C_2 s) X_L(s) = E_m(s) - \frac{K_b N_2}{K_R N_1}$$

$$E_m(s) = \left[(Ls + R) \frac{1}{K_m} (C_1 s^2 + C_2 s) + \frac{K_b N_2}{K_R N_1} \right] X_L(s)$$

$$E_m(s) = \left[\frac{(Ls + R)(C_1 s^2 + C_2 s)}{K_m} + K_m \left(\frac{K_b}{K_R} \right) \left(\frac{N_2}{N_1} \right) s \right] X_L(s)$$

$$E_m(s) = \left[\frac{s(Ls + R)(C_1 s + C_2) + K_m \left(\frac{K_b}{K_R} \right) \left(\frac{N_2}{N_1} \right)}{K_m} \right] X_L(s)$$

$$\frac{X_L(s)}{E_m(s)} = \frac{K_m}{s[(Ls + R)(C_1 s + C_2) + K_m K_b \left(\frac{N_2}{N_1} \right) \left(\frac{1}{K_R} \right)]}$$

For $\frac{X_L(s)}{D(s)} \rightarrow E_m(s) = 0$

$$(C_1 s^2 + C_2 s) X_L(s) + K_s D(s) = K_m I_a \quad \text{--- (5)}$$

from eq (1)

$$I_a(s) = \frac{-\frac{K_b}{K_R} \frac{N_2}{N_1} s}{Ls + R} X_L(s)$$

Put in (5)

(9)

$$(c_1 s^2 + c_2 s) X_2(s) + K_s D(s) = K_m \frac{-K_b \frac{N_2 s}{K_R N_1} X_2(s)}{Ls + R}$$

 $s X_2(s)$

$$\left[c_1 s^2 + c_2 s + \frac{K_m K_b \left(\frac{1}{K_R} \frac{N_2}{N_1} \right) s}{Ls + R} \right] X_2(s) + K_s D(s) = 0$$

$$\frac{s \left[(Ls + R)(c_1 s + c_2) + K_m K_b \left(\frac{1}{K_R} \frac{N_2}{N_1} \right) \right] X_2(s)}{Ls + R} = -K_s D(s)$$

$$\frac{X_2(s)}{D(s)} = \frac{-K_s (Ls + R)}{s \left[(Ls + R)(c_1 s + c_2) + K_m K_b \left(\frac{1}{K_R} \frac{N_2}{N_1} \right) \right]}$$

$$= \frac{-K_s (Ls + R)}{s \left[(Ls + R) \left(\frac{J_{\text{mot}} r}{K_R} - \frac{J_{\text{load}}}{K_R} + \frac{1}{s} m_L \right) + \left(\frac{D_1 r}{K_R} - \frac{D_2}{K_R} + K_s b \right) + \frac{K_m K_b r}{K_R} \right]}$$

$$= \frac{-K_s K_R (Ls + R)}{s \left[(Ls + R) \left((J_{\text{mot}} r - J_{\text{load}} + K_s K_R m_L) s + (D_1 r - D_2 + K_s K_R b) + K_m K_b r \right) \right]}$$

$$= \frac{-K_s K_R (Ls + R)}{s \left[(Ls + R) \left((J_{\text{mot}} r - J_{\text{load}} + K_s K_R m_L) s + (D_1 r - D_2 + K_s K_R b) + K_m K_b r \right) \right]}$$

$$K_m K_R$$

$$s \left[(Ls + R) \left((J_{\text{mot}} r - J_{\text{load}} + K_s K_R m_L) s + (D_1 r - D_2 + K_s K_R b) + K_m K_b r \right) \right]$$